backend/ConventionsC.v
@@ -1,0 +1,40 @@
+Require Import CoqlibC.
+Require Import ASTC.
+Require Import LocationsC.
+Require Export Conventions1.
+(* newly added *)
+Require Export Conventions.
+
+Local Opaque Z.add Z.mul Z.divide list_nth_z.
+Lemma tailcall_size_aux
+      tys ir fr
+      (TAIL: forall l,
+          In l (regs_of_rpairs (loc_arguments_64 tys ir fr 0)) ->
+          match l with
+          | R _ => True
+          | S _ _ _ => False
+          end)
+      (IRBOUND: (ir - 1) < list_length_z int_param_regs)
+      (FRBOUND: (fr - 1) < list_length_z float_param_regs)
+  :
+    <<SZ: size_arguments_64 tys ir fr 0 = 0>>
+.
+Proof.
+  ginduction tys; ii; ss.
+  destruct a; des_ifs; ss;
+    try (by exploit TAIL; eauto; ss);
+    (eapply IHtys; eauto;
+     [ii; des_ifs; []; exploit TAIL; eauto
+     |rewrite Z.add_simpl_r; apply list_nth_z_range in Heq; xomega]).
+Qed.
+
+Lemma tailcall_size
+      sg
+      (TAIL: tailcall_possible sg)
+  :
+    size_arguments sg = 0
+.
+Proof.
+  eapply tailcall_size_aux; eauto; cbn; xomega.
+Qed.
+
