backend/SeparationC.v
@@ -1,0 +1,29 @@
+Require Import Setoid Program.Basics.
+Require Import CoqlibC Decidableplus.
+Require Import AST Integers Values Memory Events Globalenvs.
+(** newly added **)
+Require Export Separation.
+
+Local Open Scope sep_scope.
+
+
+
+
+Section INJ.
+
+Context `{Val.meminj_ctx}.
+
+Lemma separation_private
+      m_src m_tgt F P
+      (MATCH: m_tgt |= P ** minjection F m_src)
+  :
+     P.(m_footprint) <2= loc_out_of_reach F m_src
+.
+Proof.
+  inv MATCH. des; ss.
+  ii. unfold disjoint_footprint in *. ss.
+  eapply H2; eauto.
+Qed.
+
+End INJ.
+
